\documentclass[main.tex]{subfiles}
\begin{document}
From (3.78) and (3.79),
$$
M^{-1} K=\left(\begin{array}{cc}
g / \ell+\kappa / m & -\kappa / m \\
-\kappa / m & g / \ell+\kappa / m
\end{array}\right) .
$$
The matrix $M^{-1} K-\omega^2 I$ is
$$
M^{-1} K-\omega^2 I=\left(\begin{array}{cc}
g / \ell+\kappa / m-\omega^2 & -\kappa / m \\
-\kappa / m & g / \ell+\kappa / m-\omega^2
\end{array}\right) .
$$
To find the eigenvalues of $M^{-1} K$, we form the determinant
$$
\begin{gathered}
\operatorname{det}\left[M^{-1} K-\omega^2 I\right]=\operatorname{det}\left[\left(\begin{array}{cc}
g / \ell+\kappa / m-\omega^2 & -\kappa / m \\
-\kappa / m & g / \ell+\kappa / m-\omega^2
\end{array}\right)\right] \\
=\left(g / \ell+\kappa / m-\omega^2\right)^2-(\kappa / m)^2 \\
=\left(\omega^2-g / \ell\right)\left(\omega^2-g / \ell-2 \kappa / m\right)=0 .
\end{gathered}
$$
Thus the angular frequencies of the normal modes are
$$
\omega_1^2=g / \ell, \quad \omega_2^2=g / \ell+2 \kappa / m .
$$
\end{document}